Auxiliary/Example.dfy
@@ -8,10 +8,24 @@ ghost function fib(n:int) : int
   else fib(n-1) + fib(n-2)
 }
 
-lemma {:induction n} fibOddOddEven(n:int)
+/*lemma {:induction n} fibOddOddEven(n:int)
   requires n >= 1 && n % 3 == 1
   ensures fib(n) % 2 == 1 &&  fib(n + 1) % 2 == 1 && fib(n + 2) % 2 == 0
-{}
+{}*/
+lemma fibOddOddEven(n:int)
+  requires n >= 1 && n % 3 == 1
+  ensures fib(n) % 2 == 1 &&  fib(n + 1) % 2 == 1 && fib(n + 2) % 2 == 0
+  decreases n
+{
+  if n == 1 {
+    assert fib(1) == 1 && fib(2) == 1 && fib(3) == 2;
+  }
+  else {
+    assert n >= 4;
+    assert (n - 3) % 3 == 1;
+    fibOddOddEven(n - 3);
+  }
+}
 
 method Fibonacci(n:int) returns (r:int)
   requires n >= 0
